proof/correctness/TreehashProof.ec
@@ -13,8 +13,6 @@ require import Params XMSS_MT_Params Types Address BaseW WOTS LTree XMSS_MT_Tree
 require import XMSS_IMPL Parameters.
 require import Repr2 Utils2.
 
-require import Termination.
-
 require import Array8 Array11 Array32 Array320 Array352.
 
 require import Correctness_Address.
@@ -27,25 +25,41 @@ require import Correctness_Address.
 
 (* _stack{1} = W8.t Array352.t *)
 (* For this proof, the address will be the zero address *)
-lemma treehash_correct (_auth_path : W8.t Array320.t, _sk_seed _pub_seed : W8.t Array32.t,
-                        _idx:W32.t, _addr:W32.t Array8.t) : 
+
+
+
+(* arg{1}
+
+root:W8.t Array32.t
+sk_seed:W8.t Array32.t,
+pub_seed:W8.t Array32.t, 
+s:W32.t, 
+target_height:W32.t,
+subtree_addr:W32.t Array8.t
+
+*)
+
+(* This only works for kg because of  arg{2}.`3 = 0 /\ arg{2}.`4 = h *)
+lemma treehash_correct ( _sk_seed _pub_seed : W8.t Array32.t, _s _t:W32.t, _addr:W32.t Array8.t): 
     n = XMSS_N /\
     d = XMSS_D /\
     h = XMSS_FULL_HEIGHT =>
     equiv [
       M(Syscall).__treehash ~ TreeHash.treehash :
-      arg{1}.`2 = _auth_path /\
-      arg{1}.`3 = _sk_seed /\
-      arg{1}.`4 = _pub_seed /\
-      arg{1}.`5 = _idx /\
+      arg{1}.`2 = _sk_seed /\
+      arg{1}.`3 = _pub_seed /\
+      arg{1}.`4 = _s /\
+      arg{1}.`5 = _t /\
       arg{1}.`6 = _addr /\
       arg{2}.`1 = NBytes.insubd (to_list _pub_seed) /\
       arg{2}.`2 = NBytes.insubd (to_list _sk_seed) /\
       arg{2}.`3 = 0 /\
       arg{2}.`4 = h /\
-      arg{2}.`5 = _addr
+      arg{2}.`5 = _addr /\
+
+      0 <= to_uint _t <= XMSS_TREE_HEIGHT
       ==>
-      to_list res{1}.`1 = val res{2}
+      to_list res{1} = val res{2}
     ].
 proof.
 rewrite /XMSS_N /XMSS_D /XMSS_FULL_HEIGHT => [#] n_val d_val h_val.
@@ -65,89 +79,175 @@ seq 1 0 : (#pre /\ node_addr{1}= zero_addr).
   + inline {1} 1; wp.
     ecall {1} (zero_addr_res ots_addr{1}).
     auto.
-seq 8 3 : (sub _stack{1} 0 32 = val node{2}); last first.
+
+seq 11 3 : (sub _stack{1} 0 32 = val node{2}); last first.
   + while {1} 
-    (
-     0 <= j{1} <= 32 /\
-     (forall (k : int), 0 <= k < j{1} => root{1}.[k] = _stack{1}.[k])
-    ) 
-    (32 - j{1}).
-       - auto => /> *. 
-         do split; 1,2,4: by smt().  
-         move => k??.
-         rewrite get_setE // /#.
-       - auto => /> &1 &2 H0. 
-         split => [/# | jL rootL *].
+    (#pre /\ 0 <= j{1} <= 32 /\
+     forall (k : int), 0 <= k < j{1} => root{1}.[k] = _stack{1}.[k])
+    (32 - j{1}); last first.
+       * auto => /> &1 &2 <-.
+         split => [/# | jL rootL].
          split => [/# | ???].
-         have ->: jL = 32 by smt(). 
-         move => ?.
-         apply (eq_from_nth witness); [by rewrite valP n_val size_to_list |].
-         rewrite size_to_list => j?.
-         rewrite get_to_list -H0 nth_sub // /#.
-seq 6 0 : (
-      auth_path{1} = _auth_path /\
-      sk_seed{1} = _sk_seed /\
-      pub_seed{1} = _pub_seed /\
-      leaf_idx{1} = _idx /\
-      subtree_addr{1} = _addr /\
-      pub_seed{2} = (insubd (to_list _pub_seed))%NBytes /\
-      sk_seed{2} = (insubd (to_list _sk_seed))%NBytes /\ 
-      address{2} = _addr /\
-      size stack{2} = h + 1 /\
-      to_uint offset{1} = offset{2} /\
-      s{2} = 0 /\ t{2} = 10 /\
+         have ->: jL = 32 by smt().
+         move => H1.
+         apply (eq_from_nth witness); first by rewrite size_sub // size_to_list.
+         rewrite size_to_list => i?.
+         rewrite get_to_list nth_sub // /#.
+       * auto => /> &hr *.
+         do split; 1,2,4: by smt().
+         move => k??.
+         rewrite get_setE /#. 
 
-      ots_addr{1}.[0] = _addr.[0] /\
-      ots_addr{1}.[1] = _addr.[1] /\ 
-      ots_addr{1}.[2] = _addr.[2] /\ 
-      ots_addr{1}.[3] = W32.zero /\
-      ots_addr{1}.[4] = W32.zero /\
-      ots_addr{1}.[5] = W32.zero /\
-      ots_addr{1}.[6] = W32.zero /\
-      ots_addr{1}.[7] = W32.zero /\
+seq 7 0 : (true). (* set appropriate condition *)
+      + inline {1}.
+        auto => />.
 
-      ltree_addr{1}.[0] = _addr.[0] /\
-      ltree_addr{1}.[1] = _addr.[1] /\ 
-      ltree_addr{1}.[2] = _addr.[2] /\ 
-      ltree_addr{1}.[3] = W32.one /\
-      ltree_addr{1}.[4] = W32.zero /\
-      ltree_addr{1}.[5] = W32.zero /\
-      ltree_addr{1}.[6] = W32.zero /\
-      ltree_addr{1}.[7] = W32.zero /\
+swap {1} 1 2.
+seq 2 0 : (#pre /\ to_uint upper_bound{1} = 2 ^ t{2}).
+      + auto => /> &1 &2.
+        rewrite (: 31 = 2^5 - 1) 1:/# and_mod //.
+        have ->: truncateu8 ((of_int (to_uint target_height{1} %% 2 ^ 5)))%W32 = 
+                 W8.of_int t{2} by admit.
+        search (`<<`).
+        rewrite shl_shlw.
+          * admit.
+        admit.
 
-      node_addr{1}.[0] = _addr.[0] /\
-      node_addr{1}.[1] = _addr.[1] /\ 
-      node_addr{1}.[2] = _addr.[2] /\ 
-      node_addr{1}.[3] = W32.of_int 2 /\
-      node_addr{1}.[4] = W32.zero /\
-      node_addr{1}.[5] = W32.zero /\
-      node_addr{1}.[6] = W32.zero /\
-      node_addr{1}.[7] = W32.zero
-); first by inline {1}; auto.
-seq 3 2 : (sub _stack{1} 0 32 = val (nth witness stack{2} (offset{2} - 1))); last by auto.
-inline M(Syscall).__gen_leaf_wots_ M(Syscall)._gen_leaf_wots M(Syscall).__gen_leaf_wots.
+
+seq 2 2: (sub _stack{1} 0 32 = val (nth witness stack{2} (offset{2} - 1))); last by auto.
+
 while (
-  to_uint idx{1} = i{2} /\
-  0 <= i{2} <= 2 ^ 10 /\
-  pk{1} = DecodeWotsPk pk{2} /\
-  to_list leaf{1} = val node{2} 
-  (* Add stuff about _stack *)
+          i{2} = to_uint i{1} /\
+          to_uint upper_bound{1} = t{2}
 ); last first.
-    + admit.
-(*
-    RHS 
-    1) set_type 0      => changes a.[3]
-    2) set_ots 1       => changes a.[4]
+    + auto => /> &1 &2 *.
+      admit.
 
-    4) Set type 1      => changes a.[3]
-    5) set_tree 1      => changes a.[1,2]
+seq 2 0 : (#pre /\ t32{1} = s{1} + i{1}); first by auto.
 
-    7) set_type 2           => changes a.[3]
-    8) set_tree_height 0    => changes a.[5]
-    9) set_tree_index i+1   => changes a.[6]
-*)
-swap {1} 2 -1.
-seq 2 2 : (#pre /\ ots_addr{1} = address{2}).
-    + inline; auto. admit.
+inline {1} M(Syscall).__gen_leaf_wots_ M(Syscall)._gen_leaf_wots M(Syscall).__gen_leaf_wots. (* Same as pkgen + ltree *)
 
+admit.
 qed.
+
+(*
+
+arg{2}:
+pub_seed sk_seed : seed, idx : W32.t, address : adrs
+
+ *)
+lemma build_auth_path_correct (_pub_seed _sk_seed : W8.t Array32.t, _idx : W32.t, a : adrs) :
+    len = XMSS_WOTS_LEN /\ 
+    n = XMSS_N /\
+    d = XMSS_D /\
+    h = XMSS_FULL_HEIGHT =>
+    equiv[
+      M(Syscall).__build_auth_path ~ TreeSig.buildAuthPath :
+      arg{1}.`2 = _sk_seed /\
+      arg{1}.`3 = _pub_seed /\
+      arg{1}.`4 = _idx /\
+      arg{1}.`5 = a /\
+
+      arg{2}.`1 = NBytes.insubd (to_list _pub_seed) /\
+      arg{2}.`2 = NBytes.insubd (to_list _sk_seed) /\
+      arg{2}.`3 = _idx /\
+      arg{2}.`4 = a /\
+
+
+      0 <= to_uint _idx < 2^XMSS_FULL_HEIGHT (* ou tree height *)
+      ==>
+      res{2} = EncodeAuthPath (to_list res{1})
+    ].
+proof.
+rewrite /XMSS_WOTS_LEN /XMSS_N /XMSS_D /XMSS_FULL_HEIGHT => [#] len_val n_val d_val h_val.
+proc => /=.
+seq 2 3 : (#pre /\ ={j} /\ j{1} = 0 /\ size authentication_path{2} = h). 
+  + auto => />; by rewrite size_nseq h_val.
+
+(* With this conseq, proving the last subgoal of the while loop becomes much easier *)
+conseq (: _ ==> 
+  to_list auth_path{1} = nbytes_flatten authentication_path{2} /\
+  size authentication_path{2} = h
+).
+  + auto => /> &1 &2 H0 H1 l r -> H.
+    (* A seta refere se a hipotese to_list `auth_path_L = nbytes_flatten `authentication_path_R *)
+    apply auth_path_eq.
+    rewrite /EncodeAuthPath /nbytes_flatten !insubdK.
+        * by rewrite /P.
+        * rewrite /P size_map size_chunk 1:/# size_nbytes_flatten /#.
+    apply (eq_from_nth witness).
+        * rewrite size_map size_chunk 1:/# size_nbytes_flatten /#.
+    rewrite H h_val => i?.
+    rewrite (nth_map witness). 
+        * rewrite size_chunk 1:/# size_nbytes_flatten /#.
+    rewrite /chunk nth_mkseq.
+        * rewrite size_nbytes_flatten /#.
+    apply nbytes_eq; apply (eq_from_nth witness); first by rewrite !valP.
+    rewrite valP n_val => j?.
+    rewrite insubdK => />.
+        * rewrite /P size_take 1:/# size_drop 1:/# size_nbytes_flatten /#.
+    rewrite nth_take 1,2:/# nth_drop 1,2:/# (nth_flatten witness n).
+        * pose P := (fun (s : W8.t list) => size s = n).
+          pose L := (map NBytes.val r).
+          rewrite -(all_nthP P L witness) /P /L size_map H h_val => k?.
+          by rewrite (nth_map witness) 1:/# valP.
+    rewrite (nth_map witness) /#.
+ 
+while ( 
+  0 <= to_uint idx{2} < 1024 /\
+
+  0 <= j{1} <= h /\ ={j} /\
+  size authentication_path{2} = h /\
+
+  idx{2} = i{1} /\
+  to_list sk_seed{1}  = val sk_seed{2} /\
+  to_list pub_seed{1} = val pub_seed{2} /\
+
+  forall (k : int), 0 <= k < n * j{1} => auth_path{1}.[k] = nth witness (nbytes_flatten authentication_path{2}) k
+); last first.
+    + auto => /> &2 *. 
+      do split; 1,4,5: by smt().
+        * by rewrite insubdK // /P size_to_list n_val.
+        * by rewrite insubdK // /P size_to_list n_val.
+        * move => authPathL authPathR j H0 H1 H2 H3 H4 ?? H5.
+          have j_val: j = h by smt().
+          clear H0 H1 H2 H3.
+          rewrite /EncodeAuthPath. 
+          apply (eq_from_nth witness); first by rewrite size_to_list size_nbytes_flatten_2 H4 n_val h_val.
+          rewrite size_to_list => i?.
+          by rewrite get_to_list H5 // n_val j_val h_val.
+seq 3 1 : (#pre /\ to_uint k{1} = k{2}); first by auto.
+seq 3 0 : (#pre /\ to_uint s{1} = k{2} * 2^j{1}).
+    + auto => /> &1 &2 *. 
+      rewrite shl_shlw 1:/# to_uint_shl 1:/#. 
+      admit.
+
+seq 1 1 : (#pre /\ to_list node{1} = val t{2}).
+    + inline {1} M(Syscall).__treehash_ M(Syscall)._treehash.
+      wp.
+      exists * sk_seed1{1}, pub_seed1{1}, s1{1}, t0{1}, subtree_addr0{1}.
+      elim * => P0 P1 P2 P3 P4.
+      call {1} (treehash_correct P0 P1 P2 P3 P4) => [/# |].
+      auto => /> &1 &2 *. admit.
+
+auto => /> &1 &2 ????H??H0???H1. 
+do split; 1,2,5,6: by smt().
+    * by rewrite size_put.
+move => k??.
+rewrite initiE 1:/# => />.
+rewrite /nbytes_flatten (nth_flatten witness n).
+   * pose P := (fun (s : W8.t list) => size s = n).
+     pose L := (map NBytes.val (put authentication_path{2} j{2} t{2})).
+     rewrite -(all_nthP P L witness) /P /L size_map size_put H h_val => j?.
+     by rewrite (nth_map witness) 1:#smt:(size_put) valP.
+rewrite (nth_map witness) 1:#smt:(size_put) nth_put 1:/#.
+case (j{2} * 32 <= k && k < j{2} * 32 + 32) => H2.
+   * rewrite ifT 1:/# -H1 get_to_list /#.
+   * rewrite ifF 1:/# H0 1:/# /nbytes_flatten (nth_flatten witness n).
+       - pose P := (fun (s0 : W8.t list) => size s0 = n).
+         pose L := (map NBytes.val authentication_path{2}).
+         rewrite -(all_nthP P L witness) /P /L size_map H h_val => j?.
+         by rewrite (nth_map witness) 1:/# valP.
+     by rewrite (nth_map witness) 1:/#.
+qed.
+ 
